Bank_Proofs.v
@@ -1,0 +1,15 @@
+Require Import Bank.
+
+Require Import Verdi.Verdi.
+
+Set Bullet Behavior "Strict Subproofs".
+
+Local Arguments update {_} {_} _ _ _ _ _ : simpl never.
+
+Section Bank_Proof.
+  Context {bank_base_params  : BaseParams}.
+  Context {bank_multi_params : MultiParams bank_base_params}.
+
+  (* TODO: Figure out imports and move proofs here *)
+
+End Bank_Proof.
